have ImplMarshalling work with the new weight-based bounds

disk-betree/Bounds.i.dfy
@@ -1,11 +1,11 @@
 module Bounds {
-  function BlockSize() : int { 8 * 1024 * 1024 }
+  function method BlockSize() : int { 8 * 1024 * 1024 }
 
-  function MaxNumChildren() : int { 32 }
-  function MaxTotalBucketWeight() : int { 8355784 }
+  function method MaxNumChildren() : int { 32 }
+  function method MaxTotalBucketWeight() : int { 8067784 }
 
-  function MaxCacheSize() : int { 70 }
+  function method MaxCacheSize() : int { 70 }
 
   // Minimum weight a bucket needs to have before we consider flushing it.
-  function FlushTriggerWeight() : int { MaxTotalBucketWeight() / 8 }
+  function method FlushTriggerWeight() : int { MaxTotalBucketWeight() / 8 }
 }
